schedulability.v
@@ -18,14 +18,13 @@ Module Schedulability.
 
       (* For any job j in schedule sched, ...*)
       Context {num_cpus: nat}.
-      Variable rate: Job -> processor num_cpus -> nat.
       Variable sched: schedule num_cpus arr_seq.
 
       Variable j: JobIn arr_seq.
 
       (* job j misses no deadline in sched if it completed by its absolute deadline. *)
       Definition job_misses_no_deadline :=
-        completed job_cost rate sched j (job_arrival j + job_deadline j).
+        completed job_cost sched j (job_arrival j + job_deadline j).
 
     End ScheduleOfJobs.
 
@@ -35,7 +34,6 @@ Module Schedulability.
       Variable job_task: Job -> sporadic_task.
     
       Context {num_cpus: nat}.
-      Variable rate: Job -> processor num_cpus -> nat.
       Variable sched: schedule num_cpus arr_seq.
 
       (* Consider any task tsk. *)
@@ -45,7 +43,7 @@ Module Schedulability.
       Definition task_misses_no_deadline :=
         forall (j: JobIn arr_seq),
           job_task j = tsk ->
-          job_misses_no_deadline rate sched j.
+          job_misses_no_deadline sched j.
 
       (* Task tsk doesn't miss its deadline before time t' iff all of its jobs don't miss
          their deadline by that time. *)
@@ -53,7 +51,7 @@ Module Schedulability.
         forall (j: JobIn arr_seq),
           job_task j = tsk ->
           job_arrival j + job_deadline j < t' ->
-          job_misses_no_deadline rate sched j.
+          job_misses_no_deadline sched j.
 
     End ScheduleOfTasks.
 
@@ -76,11 +74,10 @@ Module Schedulability.
     (* Consider any valid schedule... *)
     Context {num_cpus : nat}.
     Variable sched: schedule num_cpus arr_seq.
-    Variable rate: Job -> processor num_cpus -> nat.
 
     (* ... where jobs dont execute after completion. *)
     Hypothesis H_completed_jobs_dont_execute:
-      completed_jobs_dont_execute job_cost rate sched.
+      completed_jobs_dont_execute job_cost sched.
 
     Section SpecificJob.
 
@@ -89,13 +86,13 @@ Module Schedulability.
       
       (* ...that doesn't miss a deadline in this schedule, ... *)
       Hypothesis no_deadline_miss:
-        job_misses_no_deadline job_cost job_deadline rate sched j.
+        job_misses_no_deadline job_cost job_deadline sched j.
 
       (* the service received by j at any time t' after its deadline is 0. *)
       Lemma service_after_job_deadline_zero :
         forall t',
           t' >= job_arrival j + job_deadline j ->
-          service_at rate sched j t' = 0.
+          service_at sched j t' = 0.
       Proof.
         intros t' LE.
         rename no_deadline_miss into NOMISS,
@@ -104,7 +101,7 @@ Module Schedulability.
         apply/eqP; rewrite -leqn0.
         rewrite <- leq_add2l with (p := job_cost j).
         move: NOMISS => /eqP NOMISS; rewrite -{1}NOMISS addn0.
-        apply leq_trans with (n := service rate sched j t'.+1); last by apply EXEC.
+        apply leq_trans with (n := service sched j t'.+1); last by apply EXEC.
         unfold service; rewrite -> big_cat_nat with
                                    (p := t'.+1) (n := job_arrival j + job_deadline j);
             [rewrite leq_add2l /= | by ins | by apply ltnW].
@@ -115,7 +112,7 @@ Module Schedulability.
       Lemma cumulative_service_after_job_deadline_zero :
         forall t' t'',
           t' >= job_arrival j + job_deadline j ->
-          \sum_(t' <= t < t'') service_at rate sched j t = 0.
+          \sum_(t' <= t < t'') service_at sched j t = 0.
       Proof.
         ins; apply/eqP; rewrite -leqn0.
         rewrite big_nat_cond; rewrite -> eq_bigr with (F2 := fun i => 0);
@@ -134,7 +131,7 @@ Module Schedulability.
 
       (* ... that doesn't miss any deadline. *)
       Hypothesis no_deadline_misses:
-        task_misses_no_deadline job_cost job_deadline job_task rate sched tsk.
+        task_misses_no_deadline job_cost job_deadline job_task sched tsk.
 
       (* Then, for any valid job j of this task, ...*)
       Variable j: JobIn arr_seq.
@@ -146,7 +143,7 @@ Module Schedulability.
       Lemma service_after_task_deadline_zero :
         forall t',
           t' >= job_arrival j + task_deadline tsk ->
-          service_at rate sched j t' = 0.
+          service_at sched j t' = 0.
       Proof.
         rename H_valid_job into PARAMS; unfold valid_sporadic_job in *; des; intros t'.
         rewrite -H_job_of_task -PARAMS1.
@@ -157,7 +154,7 @@ Module Schedulability.
       Lemma cumulative_service_after_task_deadline_zero :
         forall t' t'',
           t' >= job_arrival j + task_deadline tsk ->
-          \sum_(t' <= t < t'') service_at rate sched j t = 0.
+          \sum_(t' <= t < t'') service_at sched j t = 0.
       Proof.
         rename H_valid_job into PARAMS; unfold valid_sporadic_job in *; des; intros t' t''.
         rewrite -H_job_of_task -PARAMS1.
